Integrate aesgcm128 (with one assume about hashed keys)

providers/evercrypt/fst/EverCrypt.AEAD.fst
@@ -41,7 +41,6 @@ let expand_in #a r k =
         in
         AES_stdcalls.aes128_key_expansion_stdcall k ek';
         let h1 = ST.get() in
-        // Gcm_simplify.aes_simplify3 ek' h1 (AES_s.key_to_round_keys_LE AES_s.AES_128 (Words.Seq_s.seq_nat8_to_seq_nat32_LE (Words.Seq_s.seq_uint8_to_seq_nat8 (G.reveal kv))));
         MB.blit ek' 0ul ek 0ul 176ul;
         pop_frame();
         let h2 = ST.get() in
@@ -67,7 +66,6 @@ let expand_in #a r k =
         in
         AES_stdcalls.aes256_key_expansion_stdcall k ek';
         let h1 = ST.get() in
-        // Gcm_simplify.aes_simplify3 ek' h1 (AES_s.key_to_round_keys_LE AES_s.AES_256 (Words.Seq_s.seq_nat8_to_seq_nat32_LE (Words.Seq_s.seq_uint8_to_seq_nat8 (G.reveal kv))));
         MB.blit ek' 0ul ek 0ul 240ul;
         pop_frame();
         let h2 = ST.get() in
@@ -115,60 +113,109 @@ let encrypt #a ek iv ad ad_len plain plain_len dst =
         let k_w = Words.Seq_s.seq_nat8_to_seq_nat32_LE k_nat in
         AES_s.is_aes_key_LE (vale_alg_of_alg a) k_w);
 
-      admit()
+      push_frame();
+      // Cannot pass a frozen buffer to a function that expects a regular
+      // buffer. (Or can we? Prove compatibility of preorders?). In any case, we
+      // just allocate a temporary on the stack and blit.
+      let tmp_keys = B.alloca 0uy 176ul in
+      MB.blit (EK?.ek ek) 0ul tmp_keys 0ul 176ul;      
+
+      let hkeys_b = B.alloca 0uy 160ul in
+
+      let h0 = get() in
+
+      let open Words.Seq_s in
+      let open Types_s in
+      let open Words_s in
+      let open AES_s in
+
+      let cipher = B.sub dst 0ul plain_len in
+      let tag = B.sub dst plain_len 16ul in
+
+      // The iv is modified by Vale, which the API does not allow. Hence
+      // we allocate a temporary buffer and blit the contents of the iv
+      let tmp_iv = B.alloca 0uy 16ul in
+      let h_pre = get() in
       
-      // push_frame();
-      // // Cannot pass a frozen buffer to a function that expects a regular
-      // // buffer. (Or can we? Prove compatibility of preorders?). In any case, we
-      // // just allocate a temporary on the stack and blit.
-      // let tmp_keys = B.alloca 0uy 176ul in
-      // MB.blit (EK?.ek ek) 0ul tmp_keys 0ul 176ul;      
+      MB.blit iv 0ul tmp_iv 0ul 12ul;
 
-      // let hkeys_b = B.alloca 0uy 160ul in
+      let h0 = get() in
 
-      // let h0 = get() in
+      // Some help is needed to prove that the end of the tmp_iv buffer
+      // is still 0s after blitting the contents of iv into the start of the buffer
+      let lemma_iv_eq () : Lemma 
+        (let iv_nat = Words.Seq_s.seq_uint8_to_seq_nat8 (B.as_seq h0 iv) in
+        let iv_nat = Seq.append iv_nat (Seq.create 4 0) in
+        Seq.equal
+          (Words.Seq_s.seq_uint8_to_seq_nat8 (B.as_seq h0 tmp_iv))
+          iv_nat)
+        = let iv_nat = Words.Seq_s.seq_uint8_to_seq_nat8 (B.as_seq h0 iv) in
+          let iv_nat = Seq.append iv_nat (Seq.create 4 0) in
+          let s_tmp = Words.Seq_s.seq_uint8_to_seq_nat8 (B.as_seq h0 tmp_iv) in
+          Seq.lemma_index_slice (B.as_seq h0 tmp_iv) 12 16 0;
+          Seq.lemma_index_slice (B.as_seq h0 tmp_iv) 12 16 1;
+          Seq.lemma_index_slice (B.as_seq h0 tmp_iv) 12 16 2;
+          Seq.lemma_index_slice (B.as_seq h0 tmp_iv) 12 16 3;          
+          assert (Seq.equal iv_nat s_tmp)
+          
 
-      // let open Words.Seq_s in
-      // let open Types_s in
-      // let open Words_s in
-      // let open AES_s in
+      in lemma_iv_eq ();
 
-      // let cipher = B.sub dst 0ul plain_len in
-      // let tag = B.sub dst plain_len 16ul in
-      
-      // // The iv is modified by Vale, which the API does not allow. Hence
-      // // we allocate a temporary buffer and blit the contents of the iv
-      // let iv' = B.alloca 0uy 16ul in
-      // MB.blit iv 0ul iv' 0ul 12ul;
+      assume (
+        let k = G.reveal (EK?.kv ek) in
+        let k_nat = Words.Seq_s.seq_uint8_to_seq_nat8 k in
+        let k_w = Words.Seq_s.seq_nat8_to_seq_nat32_LE k_nat in      
+        le_bytes_to_quad32 (seq_uint8_to_seq_nat8 (Seq.slice (B.as_seq h0 hkeys_b) 0 16)) == 
+          aes_encrypt_LE AES_128 k_w (Mkfour 0 0 0 0));
 
-      // assume (
-      //   let k = G.reveal (EK?.kv ek) in
-      //   let k_nat = Words.Seq_s.seq_uint8_to_seq_nat8 k in
-      //   let k_w = Words.Seq_s.seq_nat8_to_seq_nat32_LE k_nat in      
-      //   le_bytes_to_quad32 (seq_uint8_to_seq_nat8 (Seq.slice (B.as_seq h0 hkeys_b) 0 16)) == 
-      //     aes_encrypt_LE AES_128 k_w (Mkfour 0 0 0 0));
+      // These asserts prove that 4096 * (len {plain, ad}) are smaller than pow2_32
+      assert (max_length a = pow2 20 - 1);
+      assert_norm (4096 * (pow2 20 - 1) < Words_s.pow2_32);
 
-      // assume (4096 * UInt32.v plain_len < pow2_32);
-      // assume (4096 * UInt32.v ad_len < pow2_32);
+      GCMencryptOpt_stdcalls.gcm128_encrypt_opt_stdcall
+        (let k = G.reveal (EK?.kv ek) in
+        let k_nat = Words.Seq_s.seq_uint8_to_seq_nat8 k in
+        let k_w = Words.Seq_s.seq_nat8_to_seq_nat32_LE k_nat in G.hide k_w)
+        plain
+        (uint32_to_uint64 plain_len)
+        ad
+        (uint32_to_uint64 ad_len)
+        tmp_iv
+        cipher
+        tag
+        tmp_keys
+        hkeys_b;
 
-      // GCMencryptOpt_stdcalls.gcm128_encrypt_opt_stdcall
-      //   (let k = G.reveal (EK?.kv ek) in
-      //   let k_nat = Words.Seq_s.seq_uint8_to_seq_nat8 k in
-      //   let k_w = Words.Seq_s.seq_nat8_to_seq_nat32_LE k_nat in G.hide k_w)
-      //   plain
-      //   (uint32_to_uint64 plain_len)
-      //   ad
-      //   (uint32_to_uint64 ad_len)
-      //   iv'
-      //   cipher
-      //   tag
-      //   tmp_keys
-      //   hkeys_b;
-        
+      let h1 = get() in
 
-      // pop_frame();
+      // This assert is needed for z3 to pick up sequence equality for ciphertext
+      // and tag. It could be avoided if the spec returned both instead of appending them
+      assert (   
+        let kv_nat = Words.Seq_s.seq_uint8_to_seq_nat8 (G.reveal (EK?.kv ek)) in
+        let iv_nat = Words.Seq_s.seq_uint8_to_seq_nat8 (B.as_seq h0 iv) in
+        // the specification takes a seq16 for convenience, but actually discards
+        // the trailing four bytes; we are, however, constrained by it and append
+        // zeroes just to satisfy the spec
+        let iv_nat = S.append iv_nat (S.create 4 0) in
+        // `ad` is called `auth` in Vale world; "additional data", "authenticated
+        // data", potato, potato
+        let ad_nat = Words.Seq_s.seq_uint8_to_seq_nat8 (B.as_seq h0 ad) in
+        let plain_nat = Words.Seq_s.seq_uint8_to_seq_nat8 (B.as_seq h0 plain) in
+        assert (max_length a = pow2 20 - 1);
+        assert_norm (4096 * (pow2 20 - 1) < Words_s.pow2_32);
+        let cipher_nat, tag_nat =
+          GCM_s.gcm_encrypt_LE (vale_alg_of_alg a) kv_nat iv_nat plain_nat ad_nat
+        in
+        Seq.equal (B.as_seq h1 cipher) (seq_nat8_to_seq_uint8 cipher_nat) /\
+        Seq.equal (B.as_seq h1 tag) (seq_nat8_to_seq_uint8 tag_nat));
 
-      // admit ()
+
+      assert (Seq.equal
+        (B.as_seq h1 dst)
+        (Seq.append (B.as_seq h1 cipher) (B.as_seq h1 tag)));
+
+      pop_frame();
+      Success
 
   | AES256_GCM -> admit()
 
@@ -192,7 +239,6 @@ let encrypt #a ek iv ad ad_len plain plain_len dst =
         tmp iv ad_len ad plain_len plain dst;
       pop_frame ();
       Success
-
 
 let decrypt #a ek iv ad ad_len cipher cipher_len dst =
   if MB.is_null (EK?.ek ek) then
